working on WAA simplifications

examples/logic/ltl/waaSimplScript.sml
@@ -4,6 +4,10 @@ open alterATheory
 
 val _ = new_theory "waaSimpl"
 
+(*
+  Reducing the amount of transitions
+*)
+
 val trans_implies_def = Define`
   trans_implies (a1,q1) (a2,q2) = a2 ⊆ a1 ∧ q1 ⊆ q2`;
 
@@ -74,10 +78,18 @@ val reduceTransSimpl_def = Define`
   reduceTransSimpl (ALTER_A s i f a trans) =
     ALTER_A s i f a (removeImplied trans)`;
 
+val REDUCE_IS_WEAK = store_thm
+  ("REDUCE_IS_WEAK",
+   ``!aut. isWeakAlterA aut ==> isWeakAlterA (reduceTransSimpl aut)``,
+   rpt strip_tac >> fs[isWeakAlterA_def] >> qexists_tac `ord`
+   >> fs[isWeakWithOrder_def] >> Cases_on `aut` >> fs[reduceTransSimpl_def]
+   >> fs[removeImplied_def] >> metis_tac[]
+  );
+
 val reduced_E_def = Define`
   reduced_E run trans word (i,q) =
     let a = $@ (\a. (a,run.E (i,q)) ∈ trans q ∧ at word i ∈ a)
-    in if ?(a',q'). (a',q') ∈ trans q ∧ trans_implies (a',q') (a,run.E (i,q))
+    in if ?a' q'. (a',q') ∈ trans q ∧ trans_implies (a',q') (a,run.E (i,q))
        then SND
         ($@ \t. (t ∈ minimal_elements
                     (trans q)
@@ -92,14 +104,19 @@ val reduced_run_def = Define`
 val REDUCE_TRANS_CORRECT = store_thm
   ("REDUCE_TRANS_CORRECT",
    ``!aut. FINITE aut.states ∧ FINITE aut.alphabet ∧ isValidAlterA aut
+         ∧ isWeakAlterA aut
       ==> (alterA_lang aut = alterA_lang (reduceTransSimpl aut))``,
    rw[SET_EQ_SUBSET, SUBSET_DEF] >> rpt strip_tac >> fs[alterA_lang_def]
     >- (qexists_tac `reduced_run run x aut.trans` >> fs[runForAA_def]
+        >> `(validAARunFor (reduceTransSimpl aut) (reduced_run run x aut.trans) x ∧
+           (validAARunFor (reduceTransSimpl aut) (reduced_run run x aut.trans) x
+             ==> acceptingAARun (reduceTransSimpl aut) (reduced_run run x aut.trans))) ∧
+                    word_range x ⊆ (reduceTransSimpl aut).alphabet` suffices_by fs[]
         >> rpt strip_tac
         >> `!i. (reduced_run run x aut.trans).V i ⊆ run.V i` by (
              Induct_on `i` >> simp[SUBSET_DEF] >> rpt strip_tac
              >> fs[reduced_run_def, run_restr_def, run_restr_V_def,reduced_E_def]
-             >> Cases_on `∃(a',q').
+             >> Cases_on `∃a' q'.
                          (a',q') ∈ aut.trans q ∧
                          trans_implies (a',q')
                          ((@a. (a,run.E (i,q)) ∈ aut.trans q ∧ at x i ∈ a),
@@ -116,7 +133,7 @@ val REDUCE_TRANS_CORRECT = store_thm
                    >> HO_MATCH_MP_TAC TRANS_IMPL_MIN_LEMM >> fs[]
                  )
                    >> Cases_on `$@ minE`
-                   >> `minE (q',r)` by metis_tac[SELECT_THM]
+                   >> `minE (q'',r)` by metis_tac[SELECT_THM]
                    >> qunabbrev_tac `minE`
                    >> fs[minimal_elements_def, rrestrict_def, rel_to_reln_def]
                    >> fs[validAARunFor_def,trans_implies_def]
@@ -154,58 +171,451 @@ val REDUCE_TRANS_CORRECT = store_thm
                         )
                        >> fs[run_restr_def]
                        >> Cases_on `$@ minE` >> fs[SND]
-                       >> `minE (q'',r)` by metis_tac[SELECT_THM]
+                       >> `minE (q''',r)` by metis_tac[SELECT_THM]
                        >> qunabbrev_tac `minE` >> fs[minimal_elements_def,rrestrict_def]
                        >> fs[rel_to_reln_def, trans_implies_def]
-                       >> qabbrev_tac `a'' =
+                       >> qabbrev_tac `a''' =
                               (@a. (a,run.E (i,q)) ∈ aut.trans q ∧ at x i ∈ a)`
-                       >> `(a'', run.E (i,q)) ∈ aut.trans q ∧ at x i ∈ a''` by (
+                       >> `(a''', run.E (i,q)) ∈ aut.trans q ∧ at x i ∈ a'''` by (
                             fs[validAARunFor_def]
                             >> `q ∈ run.V i` by metis_tac[SUBSET_DEF]
                             >> metis_tac[SELECT_THM,IN_DEF]
                         )
-                       >- (qexists_tac `q''` >> Cases_on `aut` >> fs[reduceTransSimpl_def]
+                       >- (qexists_tac `q'''` >> Cases_on `aut` >> fs[reduceTransSimpl_def]
                            >> fs[removeImplied_def]
                            >> rpt strip_tac
                             >- (CCONTR_TAC >> fs[] >> metis_tac[])
                             >- metis_tac[SUBSET_TRANS,SUBSET_DEF])
-                       >- (`∃(a',q'). (a',q') ∈ aut.trans q ∧ a'' ⊆ a' ∧ q' ⊆ run.E (i,q)`
-                            suffices_by metis_tac[] >> rpt strip_tac
-                            >> simp[PEXISTS_THM] >> qexists_tac `(a'',run.E (i,q))`)
-
+                       >- metis_tac[]
                       )
-                   >- (fs[] >> rw[]
-                         >- (Cases_on `aut` >> fs[validAARunFor_def, reduceTransSimpl_def]
-                             >> fs[removeImplied_def] >> `q ∈ run.V i` by fs[SUBSET_DEF]
-                             >> `∃a. (a,run.E (i,q)) ∈ f3 q ∧ at x i ∈ a` by fs[]
-                             >> qabbrev_tac `a'' =
-                                  (@a. (a,run.E (i,q)) ∈ f3 q ∧ at x i ∈ a)`
-                             >> `(a'', run.E (i,q)) ∈ f3 q ∧ at x i ∈ a''`
-                                   by metis_tac[SELECT_THM,IN_DEF]
-                             >> qexists_tac `a''` >> fs[]
-                             >> strip_tac >> Cases_on `t'` >> CCONTR_TAC
-                             >> fs[]
-                             >> metis_tac[PEXISTS_T]
+                   >- (simp[] >> fs[run_restr_def] >> simp[]
+                       >> Cases_on `aut` >> simp[reduceTransSimpl_def, removeImplied_def]
+                       >> `?a. (a, run.E (i,q)) ∈ f3 q ∧ at x i ∈ a` by (
+                              fs[validAARunFor_def] >> metis_tac[SUBSET_DEF]
+                        )
+                       >> qabbrev_tac `a' = (@a. (a,run.E (i,q)) ∈ f3 q ∧ at x i ∈ a)`
+                       >> `(a', run.E (i,q)) ∈ f3 q ∧ at x i ∈ a'` by metis_tac[SELECT_THM]
+                       >> qexists_tac `a'` >> rpt strip_tac >> fs[]
+                       >> Cases_on `t'` >> metis_tac[]
+                      )
+                 )
+              >- (simp[SUBSET_DEF, reduced_run_def] >> rpt strip_tac
+                  >> fs[run_restr_def, run_restr_E_def]
+                  >> rw[run_restr_V_def, DECIDE ``i + 1 = SUC i``]
+                  >> metis_tac[MEMBER_NOT_EMPTY]
+                 )
+              >- (Cases_on `i = 0` >> fs[]
+                  >> `?j. i = SUC j` by (Cases_on `i` >> fs[])
+                  >> fs[reduced_run_def, run_restr_def, run_restr_V_def]
+                  >> simp[run_restr_E_def]
+                  >> metis_tac[]
+                 )
+            )
+         >- (`∀b f. infBranchOf (reduced_run run x aut.trans) b
+                ∧ branchFixP b f ⇒ f ∉ (reduceTransSimpl aut).final` suffices_by (
+                 `isWeakAlterA (reduceTransSimpl aut)` by metis_tac[REDUCE_IS_WEAK]
+                 >> `FINITE (reduceTransSimpl aut).states` by
+                      (Cases_on `aut` >> fs[reduceTransSimpl_def])
+                 >> metis_tac[BRANCH_ACC_LEMM]
+             )
+             >> `∀b f. infBranchOf run b ∧ branchFixP b f ⇒ f ∉ aut.final`
+                by metis_tac[BRANCH_ACC_LEMM]
+             >> `!b. infBranchOf (reduced_run run x aut.trans) b
+                ==> infBranchOf run b` by (
+                rpt strip_tac >> simp[infBranchOf_def] >> rpt strip_tac
+                    >- metis_tac[infBranchOf_def,SUBSET_DEF]
+                    >- (`!i. b i ∈ run.V i` by (
+                          rpt strip_tac >> fs[infBranchOf_def,validAARunFor_def]
+                          >> Cases_on `i = 0` >> fs[SUBSET_DEF]
+                          >> `?j. i = j + 1` by (
+                              Cases_on `i` >> metis_tac[SUC_ONE_ADD, ADD_COMM]
+                          )
+                          >> metis_tac[]
+                        )
+                        >> POP_ASSUM mp_tac >> POP_ASSUM mp_tac
+                        >> simp[infBranchOf_def, reduced_run_def]
+                        >> simp[run_restr_def, run_restr_E_def] >> rpt strip_tac
+                        >> POP_ASSUM mp_tac
+                        >> first_x_assum (qspec_then `i` mp_tac) >> rpt strip_tac
+                        >> `b (i+1) ∈ reduced_E run aut.trans x (i, b i)`
+                           by metis_tac[MEMBER_NOT_EMPTY]
+                        >> POP_ASSUM mp_tac >> simp[reduced_E_def] >> rpt strip_tac
+                        >> Cases_on `∃a' q'.
+                                      (a',q') ∈ aut.trans (b i) ∧
+                                      trans_implies (a',q')
+                                      ((@a. (a,run.E (i,b i)) ∈ aut.trans (b i)
+                                            ∧ at x i ∈ a),
+                                       run.E (i,b i))`
+                          >- (fs[]
+                              >> qabbrev_tac `minE = \t.
+                                    t ∈
+                                      minimal_elements (aut.trans (b i))
+                                      (rrestrict (rel_to_reln trans_implies)
+                                                 (aut.trans (b i))) ∧
+                                      trans_implies t
+                                      ((@a. (a,run.E (i,b i)) ∈ aut.trans (b i)
+                                            ∧ at x i ∈ a),
+                                       run.E (i,b i))`
+                              >> `?t. minE t` by (
+                                   qunabbrev_tac `minE` >> fs[]
+                                   >> HO_MATCH_MP_TAC TRANS_IMPL_MIN_LEMM >> fs[]
+                               )
+                              >> `minE ($@ minE)` by metis_tac[SELECT_THM]
+                              >> Cases_on `$@ minE`
+                              >> `r ⊆ run.E (i,b i)` suffices_by metis_tac[SUBSET_DEF,SND]
+                              >> qunabbrev_tac `minE` >> fs[minimal_elements_def]
+                              >> fs[rrestrict_def, rel_to_reln_def,trans_implies_def]
+                             )
+                          >- metis_tac[]
+                       )
+             )
+             >> rpt strip_tac >> `f ∈ aut.final` suffices_by metis_tac[]
+             >> Cases_on `aut` >> fs[reduceTransSimpl_def]
+            )
+         >- (Cases_on `aut` >> fs[reduceTransSimpl_def])
+       )
+    >- (qexists_tac `run` >> fs[runForAA_def]
+        >> `(validAARunFor aut run x ∧ (validAARunFor aut run x ==> acceptingAARun aut run))
+          ∧ word_range x ⊆ aut.alphabet` suffices_by fs[]
+        >> rpt strip_tac
+         >- (simp[validAARunFor_def] >> rpt strip_tac
+             >- (Cases_on `aut` >> fs[validAARunFor_def, reduceTransSimpl_def])
+             >- (Cases_on `aut` >> fs[validAARunFor_def, reduceTransSimpl_def])
+             >- (Cases_on `aut` >> fs[validAARunFor_def, reduceTransSimpl_def]
+                 >> metis_tac[removeImplied_def,IN_DIFF])
+             >- (Cases_on `aut` >> fs[validAARunFor_def, reduceTransSimpl_def])
+             >- (Cases_on `aut` >> fs[validAARunFor_def, reduceTransSimpl_def])
+            )
+         >- (`∀b x. infBranchOf run b ∧ branchFixP b x ⇒ x ∉ aut.final`
+               suffices_by metis_tac[BRANCH_ACC_LEMM]
+             >> `FINITE (reduceTransSimpl aut).states` by
+                    (Cases_on `aut` >> fs[reduceTransSimpl_def])
+             >> `aut.final = (reduceTransSimpl aut).final` by
+                  (Cases_on `aut` >> fs[reduceTransSimpl_def])
+             >> metis_tac[BRANCH_ACC_LEMM,REDUCE_IS_WEAK]
+            )
+         >- (Cases_on `aut` >> fs[reduceTransSimpl_def])
+       )
+  );
+
+(*
+  Remove unreachable states
+*)
+
+val nStepReachable_def = Define`
+   (nStepReachable trans init 0 = init)
+ ∧ (nStepReachable trans init (SUC i) =
+    {s | ?a qs s'. (a, qs) ∈ trans s' ∧ s' ∈ nStepReachable trans init i
+          ∧ s ∈ qs})`;
+
+val reachable_def = Define`
+  (reachable trans init = {s | ?n. s ∈ nStepReachable trans init n })`;
+
+val removeStatesSimpl_def = Define`
+  removeStatesSimpl (ALTER_A s i f a t) =
+            (ALTER_A (s ∩ reachable t (BIGUNION i)) i f a t)`;
+
+val REDUCE_STATE_CORRECT = store_thm
+  ("REDUCE_STATE_CORRECT",
+   ``!aut. alterA_lang aut = alterA_lang (removeStatesSimpl aut)``,
+   rw[SET_EQ_SUBSET,SUBSET_DEF] >> rpt strip_tac >> fs[alterA_lang_def]
+     >- (qexists_tac `run` >> fs[runForAA_def] >> rpt strip_tac
+          >- (simp[validAARunFor_def] >> rpt strip_tac
+             >- (Cases_on `aut` >> fs[validAARunFor_def, removeStatesSimpl_def])
+             >- (Cases_on `aut` >> fs[validAARunFor_def, removeStatesSimpl_def]
+                 >> `!n. run.V n ⊆ reachable f3 (BIGUNION f0)` by (
+                      Induct_on `n`
+                      >- (fs[reachable_def, nStepReachable_def]
+                          >> simp[SUBSET_DEF] >> rpt strip_tac
+                          >> qexists_tac `0` >> simp[nStepReachable_def]
+                          >> metis_tac[]
+                         )
+                      >- (simp[SUBSET_DEF,reachable_def] >> rpt strip_tac
+                          >> fs[reachable_def]
+                          >> `!x. x ∈ run.V n ==> ?n. x ∈ nStepReachable f3 (BIGUNION f0) n`
+                              by fs[SUBSET_DEF]
+                          >> first_x_assum (qspec_then `SUC n` mp_tac) >> rpt strip_tac
+                          >> first_x_assum (qspec_then `x'` mp_tac) >> rpt strip_tac
+                          >> fs[] >> `∃q'. x' ∈ run.E (n,q') ∧ q' ∈ run.V n` by fs[]
+                          >> `∃n. q' ∈ nStepReachable f3 (BIGUNION f0) n` by fs[]
+                          >> qexists_tac `SUC n'` >> simp[nStepReachable_def]
+                          >> metis_tac[]
+                         )
+                  ) >> fs[]
+                )
+             >- (Cases_on `aut` >> fs[validAARunFor_def, removeStatesSimpl_def])
+             >- (Cases_on `aut` >> fs[validAARunFor_def, removeStatesSimpl_def])
+             >- (Cases_on `aut` >> fs[validAARunFor_def, removeStatesSimpl_def])
+             )
+          >- (Cases_on `aut` >> fs[acceptingAARun_def, removeStatesSimpl_def])
+          >- (Cases_on `aut` >> fs[removeStatesSimpl_def])
+        )
+     >- (qexists_tac `run` >> fs[runForAA_def] >> rpt strip_tac
+         >- (simp[validAARunFor_def] >> rpt strip_tac
+             >> Cases_on `aut`
+             >> fs[validAARunFor_def, removeStatesSimpl_def])
+         >- (Cases_on `aut` >> fs[acceptingAARun_def,removeStatesSimpl_def])
+         >- (Cases_on `aut` >> fs[removeStatesSimpl_def])
+        )
+  );
+
+(*
+  Merge equivalent states
+*)
+
+val equivalentStates_def = Define`
+  equivalentStates final trans s s' =
+            (trans s = trans s') ∧ (s ∈ final = s' ∈ final)`;
+
+val replaceSingleTrans_def = Define`
+  replaceSingleTrans s s' (a,e) =
+            if s ∈ e
+            then (a, (e DIFF {s}) ∪ {s'})
+            else (a,e)`;
+
+val replaceState_def = Define`
+  replaceState s s' qs =
+                 if s ∈ qs
+                 then qs DIFF {s} ∪ {s'}
+                 else qs`;
+
+val REPL_STATE_LEMM = store_thm
+  ("REPL_STATE_LEMM",
+   ``!x s d1 d2. d1 ⊆ d2 ==> replaceState x s d1 ⊆ replaceState x s d2``,
+   rpt strip_tac >> fs[replaceState_def] >> Cases_on `x ∈ d1`
+   >> Cases_on `x ∈ d2` >> fs[SUBSET_DEF, IN_DIFF, IN_UNION] >> rpt strip_tac
+   >> metis_tac[]
+  );
+
+val replaceBy_def = Define`
+  replaceBy trans s s' q = IMAGE (replaceSingleTrans s s') (trans q)`;
+
+val mergeState_def = Define`
+  mergeState x (ALTER_A states i f a trans) =
+            if ?s. s ∈ states ∧ ~(s = x) ∧ equivalentStates f trans s x
+            then
+                let s' = $@ (\s. s ∈ states ∧ ~(s = x)
+                              ∧ equivalentStates f trans s x)
+                in ALTER_A
+                       (states DIFF {x})
+                       (IMAGE (replaceState x s') i)
+                       (replaceState x s' f)
+                       a
+                       (replaceBy trans x s')
+            else (ALTER_A states i f a trans)`;
+
+val mergeStatesSimpl = Define`
+  mergeStatesSimpl aut = ITSET mergeState aut.states aut`;
+
+(* val MERGE_STATE_COMMUTES = store_thm *)
+(*  ("MERGE_STATE_COMMUTES", *)
+(*   ``!f x y z. mergeState f x (mergeStates f y z) = *)
+(*                  mergeState f y (mergeState f x z)``, *)
 
 
+(* val ITSET_IND_SPEC_MERGE = store_thm *)
+(*   ("ITSET_IND_SPEC_MERGE", *)
+(*   ``∀P. *)
+(*   (∀s b. *)
+(*     (FINITE s ∧ s ≠ ∅ ⇒ P (REST s) ((mergeState final) (CHOICE s) b)) ⇒ P s b) ⇒ *)
+(*   ∀v v1. P v v1``, *)
+(*   metis_tac[ITSET_IND] *)
+(*   ); *)
+
+(* val EQUIV_EXISTS_IN_MERGESET = store_thm *)
+(*   ("EQUIV_EXISTS_IN_MERGESET", *)
+(*    ``!final states trans x. FINITE states ∧ (x ∈ states) *)
+(*   ==> ?x'. (x' ∈ FST (mergeStates final states trans)) *)
+(*          ∧ (equivalentStates final trans x x')``, *)
+(*      simp[mergeStates_def] >> gen_tac *)
+(*      >> `!v v1 trans. FINITE v ==> *)
+(*           !x. x ∈ v ==> *)
+(*           ?x'. x' ∈ FST (ITSET (mergeState final) v v1) ∧ *)
+(*           equivalentStates final trans x x'` by ( *)
+(*          HO_MATCH_MP_TAC ITSET_IND_SPEC_MERGE >> rpt strip_tac *)
+(*          >> `∀trans x. *)
+(*               x ∈ REST v ⇒ *)
+(*               ∃x'. x' ∈ FST *)
+(*                 (ITSET (mergeState final) (REST v) *)
+(*                        (mergeState final (CHOICE v) v1)) ∧ *)
+(*                 equivalentStates final trans x x'` *)
+(*               by metis_tac[MEMBER_NOT_EMPTY] *)
+(*          >> Cases_on `x ∈ REST v` *)
+(*            >- metis_tac[ITSET_THM,MEMBER_NOT_EMPTY] *)
+(*            >- (rw[ITSET_THM] >> fs[MEMBER_NOT_EMPTY] *)
+(*                  >- (Cases_on `v1` >> simp[mergeState_def] *)
+(*                      >> Cases_on `∃s. *)
+(*                             s ∈ q ∧ (s ≠ CHOICE v) *)
+(*                             ∧ equivalentStates final r s (CHOICE v)` *)
+(*                       >- (rw[] >> metis_tac[]) *)
+(* ) *)
+
+(* ) *)
+(*      >> HO_MATCH_MP_TAC ITSET_IND_SPEC_MERGE >> rpt strip_tac *)
+(*      >> Cases_on `(states = {})` *)
+(*        >- (simp[ITSET_THM] >> metis_tac[MEMBER_NOT_EMPTY]) *)
+(*        >- (fs[] *)
+(*            >>  *)
+(*            >>  *)
+
+(* ) *)
+
+(*    `!states. FINITE states ==> *)
+(*          !final trans x. (x ∈ states) *)
+(*          ==> ?x'. (x' ∈ FST (mergeStates final states trans)) *)
+(*          ∧ (equivalentStates final trans x x')` suffices_by metis_tac[] *)
+(*    >> Induct_on `states` >> rpt strip_tac >> fs[mergeStates_def] *)
+(*      >- () *)
+
+
+(* ) *)
+
+val replace_run_def = Define`
+  replace_run old_run x_old x_new =
+    ALTERA_RUN
+        (replaceState x_old x_new o old_run.V)
+        (λ(i,q). if (q = x_new) ∧ ~(x_new ∈ old_run.V i)
+                 then replaceState x_old x_new (old_run.E (i,x_old))
+                 else replaceState x_old x_new (old_run.E (i,q)))`;
+
+val MERGE_STATE_CORRECT = store_thm
+  ("MERGE_STATE_CORRECT",
+  ``!aut x. x ∈ aut.states ==>
+       (alterA_lang aut = alterA_lang (mergeState x aut))``,
+  rw[SET_EQ_SUBSET,SUBSET_DEF] >> rpt strip_tac >> fs[alterA_lang_def]
+  >> rename[`word_range x'`]
+    >- (`word_range x' ⊆ (mergeState x aut).alphabet` by
+           (Cases_on `aut` >> fs[mergeState_def] >> rw[COND_EXPAND_OR])
+        >> fs[]
+        >> Cases_on `∃s. s ∈ aut.states
+                ∧ s ≠ x ∧ equivalentStates aut.final aut.trans s x`
+        >- (qabbrev_tac `s' =
+              $@ (\s. s ∈ aut.states ∧ s ≠ x
+                   ∧ equivalentStates aut.final aut.trans s x)`
+            >> qexists_tac `replace_run run x s'`
+            >> fs[runForAA_def] >> rpt strip_tac
+            >> `!i q. ((q ∈ (replace_run run x s').V i) ∧ ~(q = s')
+                                                ==> (q ∈ run.V i))` by (
+                 Induct_on `i` >> fs[] >> rpt strip_tac
+                  >- (fs[replace_run_def,replaceState_def]
+                      >> Cases_on `x ∈ run.V 0` >> fs[]
+                     )
+                  >- (fs[replace_run_def, replaceState_def]
+                      >> Cases_on `x ∈ run.V (SUC i)` >> fs[]
+                     )
+             )
+            >> simp[validAARunFor_def]
+            >> rpt strip_tac
+              >- (fs[replace_run_def, replaceState_def]
+                  >> Cases_on `x ∈ run.V 0` >> fs[]
+                   >- (`s' ∈ aut.states ∧ ~(s' = x)
+                      ∧ equivalentStates aut.final aut.trans s' x`
+                         by metis_tac[SELECT_THM]
+                       >> Cases_on `aut` >> fs[mergeState_def]
+                       >> simp[] >> rw[]
+                       >- (qexists_tac `run.V 0` >> fs[validAARunFor_def]
+                           >> fs[replaceState_def]
+                          )
+                       >- metis_tac[]
+                      )
+                   >- (Cases_on `aut` >> fs[mergeState_def] >> rw[]
+                      >- (qexists_tac `run.V 0` >> fs[validAARunFor_def]
+                         >> fs[replaceState_def]
+                         )
+                      >- metis_tac[]
+                      )
+                 )
+              >- (simp[SUBSET_DEF, replace_run_def] >> rpt strip_tac
+                  >> fs[replaceState_def] >> Cases_on `x ∈ run.V i`
+                    >- (fs[]
+                        >- (Cases_on `aut` >> fs[mergeState_def]
+                            >> rw[] >> fs[validAARunFor_def]
+                            >> metis_tac[SUBSET_DEF])
+                        >- (Cases_on `aut` >> fs[mergeState_def]
+                            >> rw[] >> metis_tac[SELECT_THM])
+                       )
+                    >- (Cases_on `aut` >> fs[mergeState_def] >> rw[]
+                        >> fs[validAARunFor_def] >> metis_tac[SUBSET_DEF]
+                       )
+                 )
+              >- (simp[replace_run_def, replaceState_def]
+                  >> Cases_on `(q = s') ∧ ~(s' ∈ run.V i)` >> fs[]
+                    >- (rw[] >> fs[replace_run_def, replaceState_def]
+                        >> Cases_on `x ∈ run.V i` >> fs[]
+                        >> `?a. (a, run.E (i,x)) ∈ aut.trans x ∧ at x' i ∈ a`
+                              by metis_tac[validAARunFor_def]
+                        >> qexists_tac `a` >> fs[]
+                        >> Cases_on `aut` >> fs[mergeState_def] >> rw[]
+                               >- (simp[replaceBy_def]
+                                   >> qexists_tac `(a,run.E (i,x))`
+                                   >> fs[replaceSingleTrans_def]
+                                   >> `equivalentStates f1 f3 q x`
+                                      by metis_tac[SELECT_THM]
+                                   >> metis_tac[equivalentStates_def])
+                               >- metis_tac[]
+                               >- (simp[replaceBy_def]
+                                   >> qexists_tac `(a,run.E (i,x))`
+                                   >> fs[replaceSingleTrans_def]
+                                   >> `equivalentStates f1 f3 q x`
+                                      by metis_tac[SELECT_THM]
+                                   >> metis_tac[equivalentStates_def])
+                               >- metis_tac[]
+                       )
+                    >- (rw[] >> fs[replace_run_def, replaceState_def]
+                        >> `q ∈ run.V i` by metis_tac[IN_UNION,IN_DIFF]
+                        >> `?a. (a, run.E (i,q)) ∈ aut.trans q ∧ at x' i ∈ a`
+                                 by metis_tac[validAARunFor_def]
+                        >> qexists_tac `a` >> fs[] >> Cases_on `aut`
+                        >> fs[mergeState_def] >> rw[]
+                              >- (simp[replaceBy_def]
+                                  >> qexists_tac `(a,run.E (i,q))`
+                                  >> fs[replaceSingleTrans_def]
+                                 )
+                              >- metis_tac[]
+                              >- (simp[replaceBy_def]
+                                 >> qexists_tac `(a,run.E (i,q))`
+                                 >> fs[replaceSingleTrans_def]
+                                 )
+                       )
+                    >- (rw[] >> fs[replace_run_def, replaceState_def]
+                        >> rw[] >> `?a. (a, run.E (i,q)) ∈ aut.trans q
+                               ∧ at x' i ∈ a`
+                               by metis_tac[validAARunFor_def]
+                        >> qexists_tac `a` >> fs[] >> Cases_on `aut`
+                        >> fs[mergeState_def] >> rw[]
+                           >- (simp[replaceBy_def]
+                                >> qexists_tac `(a,run.E (i,q))`
+                                >> fs[replaceSingleTrans_def]
+                              )
+                           >- metis_tac[]
+                           >- (simp[replaceBy_def]
+                               >> qexists_tac `(a,run.E (i,q))`
+                               >> fs[replaceSingleTrans_def]
+                              )
+                       )
+                    >- (simp[replace_run_def] >> rpt strip_tac
+                        >> Cases_on `(q = s') ∧ ~(s' ∈ run.V i)` >> fs[]
+                        >> metis_tac[validAARunFor_def, REPL_STATE_LEMM]
+                       )
+                    >- (Cases_on `i = 0` >> fs[replace_run_def, replaceState_def]
+                        >> Cases_on `q = s'` >> Cases_on `x ∈ run.V i`
+                         >- (fs[]
+                             >> `?x1. x ∈ run.E (i - 1, x1)
+                                ∧ x1 ∈ run.V (i-1)` by metis_tac[validAARunFor_def]
+                             >> 
+)
+)
 
 
 )
                  )
-              >- ()
+ )
 
 
 )
-
+simp[replace_run_def,replaceState_def]
+                      >> Cases_on `aut` >> fs[mergeState_def] >> rw[]
+                       >- (fs[replaceBy_def,replaceSing])
 )
-)
-)
-
-
-)
-
-
-)
-
 
 
